builtins

minuska/theories/builtins.v
@@ -36,22 +36,10 @@ Module empty_builtin.
             : Builtin MyUnit := {|
             builtin_value
                 := Emptyset ;
-            builtin_nullary_function
+            builtin_function_symbol
                 := Emptyset ;
-            builtin_unary_function
-                := Emptyset ;
-            builtin_binary_function
-                := Emptyset ;
-            builtin_ternary_function
-                := Emptyset ;
-            builtin_nullary_function_interp
+            builtin_function_interp
                 := fun p => match p with end ;
-            builtin_unary_function_interp
-                := fun p v => match p with end ;
-            builtin_binary_function_interp
-                := fun p v1 v2 => match p with end ;
-            builtin_ternary_function_interp
-                := fun p v1 v2 v3 => match p with end ;
         |}.
 
     End sec.
@@ -77,77 +65,46 @@ Module default_builtin.
         ltac1:(solve_decision).
     Defined.
 
-    Inductive NullaryF : Set :=
-    | b_false
-    | b_true
-    | b_zero
-
-    | b_list_empty
-
-    | b_map_empty
-    .
-
-    #[export]
-    Instance NullaryF_eqDec : EqDecision NullaryF.
-    Proof. ltac1:(solve_decision). Defined.
-
-    Inductive UnaryF : Set :=
-    | b_isBuiltin (* 'a -> bool *)
-    | b_isError   (* 'a -> bool *)
-    | b_isBool    (* 'a -> bool *)
-    | b_isZ     (* 'a -> bool *)
-    | b_isString  (* 'a -> bool *)
-    | b_isList    (* 'a -> bool *)
-    | b_isMap     (* 'a -> bool *)
-
-    | b_bool_neg (* bool -> bool *)
-
-    | b_map_size    (* map -> Z *)
-    .
-
-    #[export]
-    Instance UnaryF_eqdec : EqDecision UnaryF.
-    Proof.
-        ltac1:(solve_decision).
-    Defined.
-
-    Inductive BinaryF : Set :=
-    | b_eq    (* 'a -> 'b -> bool *)
-
-    | b_and   (* bool -> bool -> bool *)
-    | b_or    (* bool -> bool -> bool *)
-    | b_iff   (* bool -> bool -> bool *)
-    | b_xor   (* bool -> bool -> bool *)
-
-    | b_Z_isLe  (* Z -> Z -> bool *)
-    | b_Z_isLt  (* Z -> Z -> bool *)
-    | b_Z_plus  (* Z -> Z -> Z *)
-    | b_Z_minus (* Z -> Z -> Z *)
-    | b_Z_times (* Z -> Z -> Z *)
-    | b_Z_div   (* Z -> Z -> Z *)
-
-    | b_map_hasKey  (* map -> 'a -> bool *)
-    | b_map_lookup  (* map -> 'a -> 'b *)
-
+    Inductive FunctionSymbol : Set :=
+    (* nulary *)
+    | b_false             (* bool *)
+    | b_true              (* bool *)
+    | b_zero              (* Z *)
+    | b_list_empty        (* list *)
+    | b_map_empty         (* map *)
+    (* unary *)
+    | b_isBuiltin         (* 'a -> bool *)
+    | b_isError           (* 'a -> bool *)
+    | b_isBool            (* 'a -> bool *)
+    | b_isZ               (* 'a -> bool *)
+    | b_isString          (* 'a -> bool *)
+    | b_isList            (* 'a -> bool *)
+    | b_isMap             (* 'a -> bool *)
+    | b_bool_neg          (* bool -> bool *)
+    | b_map_size          (* map -> Z *)
+    (* binary *)
+    | b_eq                (* 'a -> 'b -> bool *)
+    | b_and               (* bool -> bool -> bool *)
+    | b_or                (* bool -> bool -> bool *)
+    | b_iff               (* bool -> bool -> bool *)
+    | b_xor               (* bool -> bool -> bool *)
+    | b_Z_isLe            (* Z -> Z -> bool *)
+    | b_Z_isLt            (* Z -> Z -> bool *)
+    | b_Z_plus            (* Z -> Z -> Z *)
+    | b_Z_minus           (* Z -> Z -> Z *)
+    | b_Z_times           (* Z -> Z -> Z *)
+    | b_Z_div             (* Z -> Z -> Z *)
+    | b_map_hasKey        (* map -> 'a -> bool *)
+    | b_map_lookup        (* map -> 'a -> 'b *)
     | b_is_applied_symbol (* string -> 'a -> bool*)
-    | b_have_same_symbol (* term -> term -> bool*)
+    | b_have_same_symbol  (* term -> term -> bool*)
+    (* ternary*)
+    | b_map_update        (* map -> 'a -> 'b -> map  *)
     .
 
     #[export]
-    Instance BinaryF_eqdec : EqDecision BinaryF.
-    Proof.
-        ltac1:(solve_decision).
-    Defined.
-
-    Inductive TernaryF : Set :=
-    | b_map_update (* map -> 'a -> 'b -> map  *)
-    .
-
-    #[export]
-    Instance TernaryF_eqdec : EqDecision TernaryF.
-    Proof.
-        ltac1:(solve_decision).
-    Defined.
+    Instance FunctionSymbol_eqDec : EqDecision FunctionSymbol.
+    Proof. ltac1:(solve_decision). Defined.
 
     Section sec.
 
@@ -280,6 +237,57 @@ Module default_builtin.
 
         Definition my_encode := ((@encode (@TermOver' (symbol) BuiltinValue.BuiltinValue0)) _ (@TermOver_countable (symbol) BuiltinValue.BuiltinValue0 (@symbol_eqdec symbol symbols) _ (@symbol_countable symbol symbols) (@BuiltinValue.BuiltinValue0_countable (symbol) (@symbol_eqdec symbol symbols) (@symbol_countable symbol symbols)))).
 
+
+        Definition liftNulary
+            (f : MyUnit -> (@TermOver' (symbol) BuiltinValue))
+            : (MyUnit -> list (@TermOver' (symbol) BuiltinValue) -> (@TermOver' (symbol) BuiltinValue))
+        :=
+            fun nv l =>
+            match l with
+            | [] => f nv
+            | _::_ => @t_over symbol BuiltinValue (bv_error)
+            end
+        .
+
+        Definition liftUnary
+            (f : MyUnit -> (@TermOver' (symbol) BuiltinValue) -> (@TermOver' (symbol) BuiltinValue))
+            : (MyUnit -> list (@TermOver' (symbol) BuiltinValue) -> (@TermOver' (symbol) BuiltinValue))
+        :=
+            fun nv l =>
+            match l with
+            | [] => @t_over symbol BuiltinValue (bv_error)
+            | x1::[] => f nv x1
+            | _::_::_ => @t_over symbol BuiltinValue (bv_error)
+            end
+        .
+
+        Definition liftBinary
+            (f : MyUnit -> (@TermOver' (symbol) BuiltinValue) -> (@TermOver' (symbol) BuiltinValue) -> (@TermOver' (symbol) BuiltinValue))
+            : (MyUnit -> list (@TermOver' (symbol) BuiltinValue) -> (@TermOver' (symbol) BuiltinValue))
+        :=
+            fun nv l =>
+            match l with
+            | [] => @t_over symbol BuiltinValue (bv_error)
+            | _::[] => @t_over symbol BuiltinValue (bv_error)
+            | x1::x2::[] => f nv x1 x2
+            | _::_::_::_ => @t_over symbol BuiltinValue (bv_error)
+            end
+        .
+
+        Definition liftTernary
+            (f : MyUnit -> (@TermOver' (symbol) BuiltinValue) -> (@TermOver' (symbol) BuiltinValue) -> (@TermOver' (symbol) BuiltinValue) -> (@TermOver' (symbol) BuiltinValue))
+            : (MyUnit -> list (@TermOver' (symbol) BuiltinValue) -> (@TermOver' (symbol) BuiltinValue))
+        :=
+            fun nv l =>
+            match l with
+            | [] => @t_over symbol BuiltinValue (bv_error)
+            | _::[] => @t_over symbol BuiltinValue (bv_error)
+            | _::_::[] => @t_over symbol BuiltinValue (bv_error)
+            | x1::x2::x3::[] => f nv x1 x2 x3
+            | _::_::_::_::_ => @t_over symbol BuiltinValue (bv_error)
+            end
+        .
+
         #[local]
         Instance β
             : Builtin MyUnit
@@ -287,151 +295,202 @@ Module default_builtin.
             builtin_value
                 := BuiltinValue ;
 
-            builtin_nullary_function
-                := NullaryF;
+            builtin_function_symbol
+                := FunctionSymbol;
 
-            builtin_unary_function
-                := UnaryF ;
-
-            builtin_binary_function
-                := BinaryF ;
-
-            builtin_ternary_function
-                := TernaryF ;
-
-            builtin_nullary_function_interp
+            builtin_function_interp
                 := fun p =>
                 match p with
-                | b_false => fun _ => t_over (bv_bool false)
-                | b_true => fun _ => t_over (bv_bool true)
-                | b_zero => fun _ => t_over (bv_Z 0)
-                | b_list_empty => fun _ => (t_over (bv_list nil))
-                | b_map_empty => fun _ => (t_over (bv_pmap ∅))
-                end ;
- 
-            builtin_unary_function_interp
-                := fun p v =>
-                match p with
-                | b_isBuiltin => fun _ => bfmap1 impl_isBuiltin v
-                | b_isError =>
+                (* nulary *)
+                | b_false => liftNulary (
+                        fun _ => t_over (bv_bool false)
+                    )
+                | b_true => liftNulary (
+                        fun _ => t_over (bv_bool true)
+                    )
+                | b_zero => liftNulary (
+                        fun _ => t_over (bv_Z 0)
+                    )
+                | b_list_empty =>  liftNulary (
+                        fun _ => (t_over (bv_list nil))
+                    )
+                | b_map_empty =>  liftNulary (
+                        fun _ => (t_over (bv_pmap ∅))
+                    )
+                (* unary *)
+                | b_isBuiltin => liftUnary (
+                    fun _ v => bfmap1 impl_isBuiltin v
+                ) 
+                | b_isError => liftUnary (
+                    fun _ v =>
                     match v with
-                    | t_over x => fun _ => t_over (bv_bool (impl_isError x))
-                    | _ => fun _ => t_over (bv_bool false)
+                    | t_over x => t_over (bv_bool (impl_isError x))
+                    | _ => t_over (bv_bool false)
                     end
-                | b_isBool =>
+                )
+                | b_isBool => liftUnary (
+                    fun _ v =>
                     match v with
-                    | t_over x => fun _ => t_over (bv_bool (impl_isBool x))
-                    | _ => fun _ => t_over (bv_bool false)
+                    | t_over x => t_over (bv_bool (impl_isBool x))
+                    | _ => t_over (bv_bool false)
                     end
-                | b_isString =>
+                )
+                    
+                | b_isString => liftUnary (
+                    fun _ v =>
                     match v with
-                    | t_over x => fun _ => t_over (bv_bool (impl_isString x))
-                    | _ => fun _ => t_over (bv_bool false)
+                    | t_over x => t_over (bv_bool (impl_isString x))
+                    | _ => t_over (bv_bool false)
                     end
-                | b_isList =>
+                )
+                    
+                | b_isList => liftUnary (
+                    fun _ v =>
                     match v with
-                    | t_over x => fun _ => t_over (bv_bool (impl_isList x))
-                    | _ => fun _ => t_over (bv_bool false)
+                    | t_over x => t_over (bv_bool (impl_isList x))
+                    | _ => t_over (bv_bool false)
                     end
-                | b_isMap =>
+                )
+                    
+                | b_isMap => liftUnary (
+                    fun _ v =>
                     match v with
-                    | t_over x => fun _ => t_over (bv_bool (impl_isMap x))
-                    | _ => fun _ => t_over (bv_bool false)
+                    | t_over x => t_over (bv_bool (impl_isMap x))
+                    | _ => t_over (bv_bool false)
                     end
+                )
 
-                | b_bool_neg =>
-                    fun _ => bfmap_bool__bool negb v
+                | b_bool_neg => liftUnary (
+                    fun _ v =>
+                    bfmap_bool__bool negb v
+                )
                 
-                | b_isZ =>
+                | b_isZ => liftUnary (
+                    fun _ v =>
                     match v with
-                    | t_over x => fun _ => t_over (bv_bool (impl_isZ x))
-                    | _ => fun _ => t_over (bv_bool false)
+                    | t_over x => t_over (bv_bool (impl_isZ x))
+                    | _ => t_over (bv_bool false)
                     end
+                )
+                    
                 
-                | b_map_size =>
+                | b_map_size => liftUnary (
+                    fun _ v =>
                     match v with
-                    | t_over (bv_pmap m) => fun _ => (t_over (bv_Z (Z.of_nat (size m))))
-                    | _ => fun _ => err
+                    | t_over (bv_pmap m) => (t_over (bv_Z (Z.of_nat (size m))))
+                    | _ => err
                     end
-                end;
+                )
 
-            builtin_binary_function_interp
-                := fun p v1 v2 =>
-                match p with
-                | b_eq =>
-                    fun _ => t_over (bv_bool (bool_decide (v1 = v2)))
-                | b_and =>
-                    fun _ => bfmap_bool_bool__bool andb v1 v2
-                | b_or =>
-                    fun _ => bfmap_bool_bool__bool orb v1 v2
-                | b_iff =>
-                    fun _ => bfmap_bool_bool__bool eqb v1 v2
-                | b_xor =>
-                    fun _ => bfmap_bool_bool__bool xorb v1 v2                    
-                | b_Z_isLe =>
-                    fun _ => bfmap_Z_Z__bool Z.leb v1 v2
-                | b_Z_isLt =>
-                    fun _ => bfmap_Z_Z__bool Z.ltb v1 v2
-                | b_Z_plus =>
-                    fun _ => bfmap_Z_Z__Z Z.add v1 v2
-                | b_Z_minus =>
-                    fun _ => bfmap_Z_Z__Z Z.sub v1 v2
-                | b_Z_times =>
-                    fun _ => bfmap_Z_Z__Z Z.mul v1 v2
-                | b_Z_div =>
-                match v2 with
-                | t_over (bv_Z (0)) => fun _ => err
-                | _ => fun _ => bfmap_Z_Z__Z Z.div v1 v2
-                end
-                | b_map_hasKey =>
+                (* binary *)
+                | b_eq => liftBinary (
+                    fun _ v1 v2 =>
+                    t_over (bv_bool (bool_decide (v1 = v2)))
+                )
+                | b_and => liftBinary (
+                    fun _ v1 v2 =>
+                    bfmap_bool_bool__bool andb v1 v2
+                )
+                    
+                | b_or => liftBinary (
+                    fun _ v1 v2 =>
+                    bfmap_bool_bool__bool orb v1 v2
+                )
+                | b_iff => liftBinary (
+                    fun _ v1 v2 =>
+                    bfmap_bool_bool__bool eqb v1 v2
+                )
+                | b_xor => liftBinary (
+                    fun _ v1 v2 =>
+                    bfmap_bool_bool__bool xorb v1 v2
+                )
+                | b_Z_isLe => liftBinary (
+                    fun _ v1 v2 =>
+                    bfmap_Z_Z__bool Z.leb v1 v2
+                )
+                | b_Z_isLt => liftBinary (
+                    fun _ v1 v2 =>
+                    bfmap_Z_Z__bool Z.ltb v1 v2
+                )
+                | b_Z_plus => liftBinary (
+                    fun _ v1 v2 =>
+                    bfmap_Z_Z__Z Z.add v1 v2
+                )
+                | b_Z_minus => liftBinary (
+                    fun _ v1 v2 =>
+                    bfmap_Z_Z__Z Z.sub v1 v2
+                )
+                | b_Z_times => liftBinary (
+                    fun _ v1 v2 =>
+                    bfmap_Z_Z__Z Z.mul v1 v2
+                )
+                | b_Z_div => liftBinary (
+                    fun _ v1 v2 =>
+                    match v2 with
+                    | t_over (bv_Z (0)) => err
+                    | _ => bfmap_Z_Z__Z Z.div v1 v2
+                    end
+                )
+                | b_map_hasKey => liftBinary (
+                    fun _ v1 v2 =>
                     match v1 with
                     | t_over (bv_pmap m) =>
                         let p := my_encode (v2) in
                         match m !! p with
-                        | Some _ => fun _ => (t_over (bv_bool true))
-                        | None => fun _ => (t_over (bv_bool false))
+                        | Some _ => (t_over (bv_bool true))
+                        | None => (t_over (bv_bool false))
                         end
-                    | _ => fun _ => err
+                    | _ => err
                     end
-                | b_map_lookup =>
+                )
+                | b_map_lookup => liftBinary (
+                    fun _ v1 v2 =>
                     match v1 with
                     | t_over (bv_pmap m) =>
                         let p := my_encode (v2) in
                         match m !! p with
-                        | Some v => fun _ => (prettify v)
-                        | None => fun _ => err
+                        | Some v => (prettify v)
+                        | None => err
                         end
-                    | _ => fun _ => err
+                    | _ => err
                     end
-                | b_have_same_symbol =>
+                )
+                    
+                | b_have_same_symbol => liftBinary (
+                    fun _ v1 v2 =>
                     match v1 with
                     | t_term s1 _ =>
                         match v2 with
-                        | t_term s2 _ => fun _ => (t_over (bv_bool (bool_decide (s1 = s2))))
-                        | _ => fun _ => t_over (bv_bool false)
+                        | t_term s2 _ => (t_over (bv_bool (bool_decide (s1 = s2))))
+                        | _ => t_over (bv_bool false)
                         end
-                    | _ => fun _ => t_over (bv_bool false)
+                    | _ => t_over (bv_bool false)
                     end
-                | b_is_applied_symbol =>
+                )
+                    
+                | b_is_applied_symbol => liftBinary (
+                    fun _ v1 v2 =>
                     match v1 with
                     | t_over (bv_sym s) =>
                         match v2 with
-                        | t_term s' _ => fun _ => (t_over (bv_bool (bool_decide (s' = s))))
-                        | _ => fun _ => (t_over (bv_bool false))
+                        | t_term s' _ => (t_over (bv_bool (bool_decide (s' = s))))
+                        | _ => (t_over (bv_bool false))
                         end
-                    | _ => fun _ => (t_over (bv_bool false))
+                    | _ => (t_over (bv_bool false))
                     end
-                end ;
-            builtin_ternary_function_interp := fun p v1 v2 v3 =>
-                match p with
-                | b_map_update =>
+                )
+
+                (* ternary *)
+                | b_map_update => liftTernary (
+                    fun _ v1 v2 v3 =>
                     match v1 with
                     | t_over (bv_pmap m) =>
                         let p := my_encode (v2) in
                         let m' := <[ p := (uglify' v3) ]>m in
-                        fun _ => t_over (bv_pmap m')
-                    | _ => fun _ => err
+                        t_over (bv_pmap m')
+                    | _ => err
                     end
+                )
                 end ;
         |}.
 
@@ -441,108 +500,107 @@ Module default_builtin.
     Module Notations.
         
         
-        Notation "'true'" := ( (e_nullary b_true))
+        Notation "'true'" := ( (e_fun b_true []))
             : RuleScope
         .
 
-        Notation "'false'" := ( (e_nullary b_false))
+        Notation "'false'" := ( (e_fun b_false []))
             : RuleScope
         .
     
         Notation "b1 '&&' b2" :=
-            ( (e_binary default_builtin.b_and
-                ( b1)
-                ( b2)
+            ( (e_fun default_builtin.b_and
+                [b1;
+                b2]
             ))
             : RuleScope
         .
 
         Notation "b1 '||' b2" :=
-            ( (e_binary default_builtin.b_or
-                ( b1)
-                ( b2)
+            ( (e_fun default_builtin.b_or
+                [b1; b2]
             ))
             : RuleScope
         .
 
         Notation "~~ b" :=
-            ( (e_unary default_builtin.b_bool_neg ( b)))
+            ( (e_fun default_builtin.b_bool_neg [b]))
         .
 
         Notation "'isBool' t" :=
-            ( (e_unary
+            ( (e_fun
                 b_isBool
-                ( t)
+                [(t)]
             ))
             (at level 90)
         .        
 
         Notation "'isZ' t" :=
-            ((e_unary
+            ((e_fun
                 b_isZ
-                (t)
+                [(t)]
             ))
             (at level 90)
         .
 
         Notation "'isString' t" :=
-            ((e_unary
+            ((e_fun
                 b_isString
-                (t)
+                [(t)]
             ))
             (at level 90)
         .
 
         Notation "'isList' t" :=
-            ((e_unary
+            ((e_fun
                 b_isList
-                (t)
+                [(t)]
             ))
             (at level 90)
         .
 
         Notation "'isMap' t" :=
-            ((e_unary
+            ((e_fun
                 b_isMap
-                (t)
+                [(t)]
             ))
             (at level 90)
         .
 
         Notation "'(' x '+Z' y ')'" :=
-            ((e_binary b_Z_plus (x) (y)))
+            ((e_fun b_Z_plus [(x); (y)]))
         .
 
         Notation "'(' x '-Z' y ')'" :=
-            ((e_binary b_Z_minus (x) (y)))
+            ((e_fun b_Z_minus [(x); (y)]))
         .
 
         Notation "'(' x '*Z' y ')'" :=
-            ((e_binary b_Z_times (x) (y)))
+            ((e_fun b_Z_times [(x); (y)]))
         .
 
         Notation "'(' x '/Z' y ')'" :=
-            ((e_binary b_Z_div (x) (y)))
+            ((e_fun b_Z_div [(x); (y)]))
         .
 
         Notation "'(' x '<Z' y ')'" :=
-            ((e_binary b_Z_isLt (x) (y)))
+            ((e_fun b_Z_isLt [(x); (y)]))
         .
 
         Notation "'(' x '>Z' y ')'" :=
-            ((e_binary b_Z_isLt (x) (y)))
+            ((e_fun b_Z_isLt [(x); (y)]))
         .
 
         Notation "'(' x '==Z' y ')'" :=
-            ((e_binary b_eq (x) (y)))
+            ((e_fun b_eq [(x); (y)]))
         .
 
         Notation "'(' x '==Bool' y ')'" :=
-            ((e_binary b_eq (x) (y)))
+            ((e_fun b_eq [(x); (y)]))
         .
 
         Notation "'(' x '==Gen' y ')'" :=
-            ((e_binary b_eq (x) (y)))
+            ((e_fun b_eq [(x); (y)]))
         .
 
 
@@ -555,10 +613,11 @@ End default_builtin.
 
 Definition isAppliedSymbol (s:string) (e : @Expression2 (default_model (default_builtin.β))) :=
     let M := ( default_model (default_builtin.β)) in
-    ((@e_binary M
+    (@e_fun M
         default_builtin.b_is_applied_symbol
-        (@e_ground (M) (t_over (bv_sym s)))
-        )
-        (e)
+        [
+            (@e_ground (M) (t_over (bv_sym s)));
+            (e)
+        ]
     )
 .
